testing 10

LeanSAT/Reflect/CNF/Decidable.lean
@@ -18,21 +18,87 @@ For that we need to relabel in `Fin k` for some `k`.
 
 namespace CNF
 
-def Clause.maxLiteral (c : Clause Nat) : Option Nat := (c.map (·.1)) |>.minimum?
+def Clause.maxLiteral (c : Clause Nat) : Option Nat := (c.map (·.1)) |>.maximum?
+
+theorem Clause.of_maxLiteral_eq_some (c : Clause Nat) (h : c.maxLiteral = some maxLit) :
+    ∀ lit, mem lit c → lit ≤ maxLit := by
+  intro lit hlit
+  simp only [maxLiteral, List.maximum?_eq_some_iff', List.mem_map, forall_exists_index, and_imp, forall_apply_eq_imp_iff₂] at h
+  simp only [mem] at hlit
+  rcases h with ⟨_, hbar⟩
+  cases hlit
+  all_goals
+    have := hbar (lit, _) (by assumption)
+    omega
+
+theorem Clause.maxLiteral_eq_some_of_mem (c : Clause Nat) (h : mem l c) : ∃ maxLit, c.maxLiteral = some maxLit := by
+  dsimp[mem] at h
+  cases h <;> rename_i h
+  all_goals
+    have h1 := List.ne_nil_of_mem h
+    have h2 := not_congr <| @List.maximum?_eq_none_iff _ (c.map (·.1)) _
+    simp[← Option.ne_none_iff_exists', h1, h2, maxLiteral]
+
+theorem Clause.of_maxLiteral_eq_none (c : Clause Nat) (h : c.maxLiteral = none) :
+    ∀ lit, ¬mem lit c := by
+  intro lit hlit
+  simp only [maxLiteral, List.maximum?_eq_none_iff, List.map_eq_nil] at h
+  simp only [h, not_mem_nil] at hlit
 
 def maxLiteral (g : CNF Nat) : Option Nat :=
-  g.foldl (init := none) fun
-    | none, c => c.maxLiteral
-    | some m, c => match c.maxLiteral with
-      | some m' => some (max m m')
-      | none => m
+  List.filterMap Clause.maxLiteral g |>.maximum?
+
+theorem of_maxLiteral_eq_some' (c : CNF Nat) (h : c.maxLiteral = some maxLit) :
+    ∀ clause, clause ∈ c → clause.maxLiteral = some localMax → localMax ≤ maxLit := by
+  intro clause hclause1 hclause2
+  simp[maxLiteral, List.maximum?_eq_some_iff'] at h
+  rcases h with ⟨_, hclause3⟩
+  apply hclause3 localMax clause hclause1 hclause2
+
+theorem of_maxLiteral_eq_some (c : CNF Nat) (h : c.maxLiteral = some maxLit) :
+    ∀ lit, mem lit c → lit ≤ maxLit := by
+  intro lit hlit
+  dsimp[mem] at hlit
+  rcases hlit with ⟨clause, ⟨hclause1, hclause2⟩⟩
+  rcases Clause.maxLiteral_eq_some_of_mem clause hclause2 with ⟨localMax, hlocal⟩
+  have h1 := of_maxLiteral_eq_some' c h clause hclause1 hlocal
+  have h2 := Clause.of_maxLiteral_eq_some clause hlocal lit hclause2
+  omega
+
+-- TODO: probably upstream?
+theorem List.all_none_of_filterMap_eq_nil (h : List.filterMap f xs = []) : ∀ x ∈ xs, f x = none := by
+  intro x hx
+  induction xs with
+  | nil => contradiction
+  | cons y ys ih =>
+    simp [List.filterMap] at h
+    split at h
+    . cases hx with
+      | head => assumption
+      | tail _ hmem => exact ih h hmem
+    . contradiction
+
+theorem of_maxLiteral_eq_none (c : CNF Nat) (h : c.maxLiteral = none) :
+    ∀ lit, ¬mem lit c := by
+  intro lit hlit
+  simp only [maxLiteral, List.maximum?_eq_none_iff] at h
+  dsimp [mem] at hlit
+  rcases hlit with ⟨clause, ⟨hclause1, hclause2⟩⟩
+  have := Clause.of_maxLiteral_eq_none clause (List.all_none_of_filterMap_eq_nil h clause hclause1) lit
+  contradiction
 
 def numLiterals (g : CNF Nat) :=
   match g.maxLiteral with
   | none => 0
   | some n => n + 1
 
-theorem lt_numLiterals {g : CNF Nat} (h : mem a g) : a < numLiterals g := sorry
+theorem lt_numLiterals {g : CNF Nat} (h : mem a g) : a < numLiterals g := by
+  dsimp[numLiterals]
+  split <;> rename_i h2
+  . exfalso
+    apply of_maxLiteral_eq_none g h2 a h
+  . have := of_maxLiteral_eq_some g h2 a h
+    omega
 
 theorem numLiterals_pos {g : CNF Nat} (h : mem a g) : 0 < numLiterals g :=
   Nat.lt_of_le_of_lt (Nat.zero_le _) (lt_numLiterals h)
